wip
Signed-off-by: John Kastner <jkastner@amazon.com>

cedar-lean/Cedar/Thm/BatchedEvaluator.lean
@@ -6,7 +6,9 @@ import Cedar.Thm.Validation
 import Cedar.Thm.TPE
 
 /-!
-This file defines theorems related to the batched evaluator
+This file defines theorems related to the batched evaluator.
+These proofs need updating for the new RequestRefines/EntitiesRefine signatures
+and the rTargetCorrect invariant.
 -/
 
 namespace Cedar.Thm
@@ -17,166 +19,39 @@ open Cedar.Validation
 open Cedar.Thm
 open Cedar.Data
 
-
-/-- A well behaved entity loader
-1. Loads all the requested entities, returning none for missing
-entities
-2. Refines the backing entity store
-
-The first condition is required for convergence of
-batched evaluation, which has not been proven. It is unused
-in the code base at the moment.
--/
-abbrev EntityLoader.WellBehaved (store: Entities) (loader: EntityLoader) : Prop :=
+abbrev EntityLoader.WellBehaved (env : TypeEnv) (store: Entities) (loader: EntityLoader) : Prop :=
   ∀ s, s ⊆ (loader s).keys ∧
-       EntitiesRefine store ((loader s).mapOnValues MaybeEntityData.asPartial)
+       EntitiesRefine env store ((loader s).mapOnValues MaybeEntityData.asPartial)
 
-theorem as_partial_request_refines {req : Request} :
-  RequestRefines req req.asPartialRequest := by
-  simp only [Request.asPartialRequest, RequestRefines, PartialEntityUID.asEntityUID, Option.map_some]
-  constructor
-  · apply PartialIsValid.some
-    rfl
-  constructor
-  · trivial
-  constructor
-  · apply PartialIsValid.some
-    rfl
-  · apply PartialIsValid.some
-    rfl
+theorem as_partial_request_refines {req : Request} {env : TypeEnv} :
+  RequestRefines env req req.asPartialRequest := by sorry
 
-theorem any_refines_empty_entities :
-  EntitiesRefine es Data.Map.empty := by
-  simp only [EntitiesRefine, Data.Map.empty, Data.Map.find?, Map.toList]
-  intro a e₂ h₁
-  contradiction
+theorem any_refines_empty_entities {env : TypeEnv} :
+  EntitiesRefine env es Map.empty := by sorry
 
--- Helper lemma for map append refinement
-theorem entities_refine_append (es : Entities) (m1 m2 : PartialEntities) :
-  EntitiesRefine es m1 → EntitiesRefine es m2 → EntitiesRefine es (m2 ++ m1) := by
-  intro h1 h2
-  unfold EntitiesRefine
-  intro a e₂ h_find
-  rw [Map.find?_append] at h_find
-  cases h_case : m2.find? a with
-  | some e₂' =>
-    have h_eq : e₂ = e₂' := by
-      rw [h_case] at h_find
-      simp only [Option.some_or, Option.some.injEq] at h_find
-      rw [h_find]
-    rw [h_eq]
-    exact h2 a e₂' h_case
-  | none =>
-    have h_find1 : m1.find? a = some e₂ := by
-      rw [h_case] at h_find
-      simp only [Option.none_or] at h_find
-      rw [h_find]
-    exact h1 a e₂ h_find1
+theorem entities_refine_append {env : TypeEnv} (es : Entities) (m1 m2 : PartialEntities) :
+  EntitiesRefine env es m1 → EntitiesRefine env es m2 → EntitiesRefine env es (m2 ++ m1) := by sorry
 
-
-theorem direct_request_and_entities_refine (req : Request) (es : Entities) :
-  RequestAndEntitiesRefine req es req.asPartialRequest es.asPartial := by
-  constructor
-  · exact as_partial_request_refines
-  · unfold EntitiesRefine Entities.asPartial
-    intro uid data₂ h_find
-    have h_mapOnValues := Map.find?_mapOnValues_some' EntityData.asPartial h_find
-    obtain ⟨data₁, h_find₁, h_eq⟩ := h_mapOnValues
-    exists data₁
-    exact ⟨h_find₁,
-           by rw [h_eq]; apply PartialIsValid.some; rfl,
-           by rw [h_eq]; apply PartialIsValid.some; rfl,
-           by rw [h_eq]; apply PartialIsValid.some; rfl⟩
+theorem direct_request_and_entities_refine {env : TypeEnv} (req : Request) (es : Entities) :
+  RequestAndEntitiesRefine env req es req.asPartialRequest Map.empty := by sorry
 
 theorem batched_eval_loop_eq_evaluate
-  {x : Residual}
-  {req : Request}
-  (es : Entities)
-  {current_store : PartialEntities}
-  {env : TypeEnv} :
-  EntityLoader.WellBehaved es loader →
-  Residual.WellTyped env x →
-  RequestAndEntitiesRefine req es req.asPartialRequest current_store →
+  {x : TypedExpr} {req : Request} {es : Entities} {env : TypeEnv}
+  {loader : EntityLoader} {store : PartialEntities} {r : Residual} {n : Nat} :
+  Cedar.Thm.TypedExpr.WellTyped env x →
   InstanceOfWellFormedEnvironment req es env →
-  (Residual.evaluate (batchedEvalLoop x req loader current_store iters) req es).toOption = (Residual.evaluate x req es).toOption := by
-  intro h₀ h₁ h₂ h₃
-  unfold batchedEvalLoop
-  split
-  case h_1 => simp only
-  case h_2 iters n=>
-    let toLoad := (Set.filter (fun uid => (Map.find? current_store uid).isNone) x.allLiteralUIDs)
-    let newEntities := ((loader toLoad).mapOnValues MaybeEntityData.asPartial)
-    let newStore := newEntities ++ current_store
+  EntityLoader.WellBehaved env es loader →
+  EntitiesRefine env es store →
+  Residual.WellTyped env r →
+  r.evaluate req es = x.toResidual.evaluate req es →
+  (batchedEvalLoop r req loader store n).evaluate req es = x.toResidual.evaluate req es := by sorry
 
-    have h₀₂ := h₀
-    specialize h₀₂ toLoad
-    obtain ⟨h₄, h₅⟩ := h₀₂
-
-    have h₆ : RequestAndEntitiesRefine req es req.asPartialRequest newStore := by
-      unfold RequestAndEntitiesRefine
-      constructor
-      · exact as_partial_request_refines
-      · apply entities_refine_append
-        · unfold RequestAndEntitiesRefine at h₂
-          exact h₂.right
-        · apply h₅
-    let newRes := TPE.evaluate x req.asPartialRequest newStore
-    have h₇ : (Residual.evaluate newRes req es).toOption = (Residual.evaluate x req es).toOption := by
-      subst newRes
-      rw [← partial_evaluate_is_sound h₁ h₃ h₆ sorry]
-
-    simp only
-    split
-    case h_1 h₆ =>
-      rw [← h₆]
-      subst toLoad newStore newRes
-      exact h₇
-    case h_2 =>
-      subst toLoad newStore newRes
-      have h₈ := (partial_eval_preserves_well_typed h₃ h₆ h₁)
-
-      rw [batched_eval_loop_eq_evaluate es h₀ h₈ h₆ h₃]
-      exact h₇
-
-/--
-The main correctness theorem for batched evaluation:
-Batched evaluation with an entity loader produces the same result
-as normal evaluation with the complete entity store.
--/
 theorem batched_eval_eq_evaluate
-  {x : TypedExpr}
-  {req : Request}
-  {es : Entities}
-  {env : TypeEnv} :
-  EntityLoader.WellBehaved es loader →
-  TypedExpr.WellTyped env x →
+  {x : TypedExpr} {req : Request} {es : Entities} {env : TypeEnv}
+  {loader : EntityLoader} {n : Nat} :
+  Cedar.Thm.TypedExpr.WellTyped env x →
   InstanceOfWellFormedEnvironment req es env →
-  (Residual.evaluate (batchedEvaluate x req loader iters) req es).toOption = (evaluate x.toExpr req es).toOption := by
-  simp only [batchedEvaluate]
-  intro h₁ h₂ h₃
-  have h₄ := (direct_request_and_entities_refine req es)
-
-  let first_partial := (TPE.evaluate x.toResidual req.asPartialRequest (Entities.asPartial (Data.Map.mk [])))
-  let h₅ : Residual.WellTyped env (TypedExpr.toResidual x) := by {
-    apply conversion_preserves_typedness
-    exact h₂
-  }
-  rw [conversion_preserves_evaluation x req es]
-  rw [partial_evaluate_is_sound h₅ h₃ h₄ sorry]
-
-  have h₆ : Residual.WellTyped env (TPE.evaluate x.toResidual req.asPartialRequest Map.empty) := by
-    apply partial_eval_preserves_well_typed h₃ _ h₅
-    . unfold RequestAndEntitiesRefine
-      constructor
-      . apply as_partial_request_refines
-      . apply any_refines_empty_entities
-  have h₇: RequestAndEntitiesRefine req es req.asPartialRequest Map.empty := by
-    constructor
-    . apply as_partial_request_refines
-    . apply any_refines_empty_entities
-
-  rw [batched_eval_loop_eq_evaluate es h₁ h₆ h₇ h₃]
-  rw [←partial_evaluate_is_sound h₅ h₃ h₇ sorry]
-  rw [←partial_evaluate_is_sound h₅ h₃ h₄ sorry]
+  EntityLoader.WellBehaved env es loader →
+  (batchedEvaluate x req loader n).evaluate req es = x.toResidual.evaluate req es := by sorry
 
 end Cedar.Thm
